src/tls/MiTLS.HKDF.fsti
@@ -1,0 +1,135 @@
+(**
+TLS 1.3 HKDF extract and expand constructions, parametrized by their hash algorithm
+*)
+module MiTLS.HKDF
+open MiTLS
+
+open MiTLS.Mem
+
+open FStar.UInt32
+// open FStar.Integers
+// 18-09-24 still triggering extraction error
+
+open MiTLS.Hashing.Spec
+open FStar.Bytes
+
+(*-------------------------------------------------------------------*)
+(*
+From https://tools.ietf.org/html/rfc5869
+
+HKDF-Extract(salt, IKM) -> PRK
+   Options:
+      Hash     a hash function; HashLen denotes the length of the
+               hash function output in octets
+   Inputs:
+      salt     optional salt value (a non-secret random value);
+               if not provided, it is set to a string of HashLen zeros.
+      IKM      input keying material
+   Output:
+      PRK      a pseudorandom key (of HashLen octets)
+
+   PRK = HMAC-Hash(salt, IKM)
+*)
+
+inline_for_extraction
+let extract:
+  #ha: Hashing.Spec.tls_macAlg ->
+  salt: hkey ha ->
+  ikm: macable ha ->
+  ST (hkey ha)
+  (requires (fun h0 -> True))
+  (ensures (fun h0 t h1 -> FStar.HyperStack.modifies Set.empty h0 h1))
+  = fun #ha salt ikm -> HMAC.hmac ha salt ikm
+
+(*-------------------------------------------------------------------*)
+(*
+HKDF-Expand(PRK, info, L) -> OKM
+   Options:
+      Hash     a hash function; HashLen denotes the length of the
+               hash function output in octets
+   Inputs:
+      PRK      a pseudorandom key of at least HashLen octets
+               (usually, the output from the extract step)
+      info     optional context and application specific information
+               (can be a zero-length string)
+      L        length of output keying material in octets (<= 255*HashLen)
+   Output:
+      OKM      output keying material (of L octets)
+
+   N = ceil(L/HashLen)
+   T = T(1) | T(2) | T(3) | ... | T(N)
+
+   OKM = first L octets of T
+
+   where:
+   T(0) = empty string
+   T(1) = HMAC-Hash(PRK, T(0) | info | 0x01)
+   T(2) = HMAC-Hash(PRK, T(1) | info | 0x02)
+   ...
+*)
+
+val expand_spec:
+  #ha:Hashing.alg ->
+  prk: Hashing.Spec.tag ha ->
+  info: bytes {Bytes.length info < 1024 (* somewhat arbitrary *) } ->
+  len: UInt32.t {0 < v len /\ v len <= op_Multiply 255 (hash_length ha)} ->
+  GTot (lbytes32 len)
+
+val expand:
+  #ha:Hashing.Spec.tls_macAlg ->
+  prk: lbytes (Spec.Hash.Definitions.hash_length ha) ->
+  info: bytes {Bytes.length info < 1024 (* somewhat arbitrary *) } ->
+  len: UInt32.t {0 < v len /\ v len <= op_Multiply 255 (hash_length ha)} ->
+  ST (lbytes32 len)
+  (requires (fun h0 -> True))
+  (ensures (fun h0 t h1 -> modifies_none h0 h1 /\
+    t == expand_spec #ha prk info len))
+
+(*-------------------------------------------------------------------*)
+(*
+HKDF-Expand-Label(Secret, Label, Messages, Length) =
+       HKDF-Expand(Secret, HkdfLabel, Length)
+
+  Where HkdfLabel is specified as:
+
+  struct HkdfLabel {
+    uint16 length;
+    opaque label<9..255>;
+    opaque hash_value<0..255>;
+  };
+
+  - HkdfLabel.length is Length
+  - HkdfLabel.label is "TLS 1.3, " + Label
+  - HkdfLabel.hash_value is HashValue.
+*)
+
+/// used for computing all derived keys; 
+
+val expand_label:
+  #ha: Hashing.Spec.tls_macAlg ->
+  secret: lbytes (Spec.Hash.Definitions.hash_length ha) ->
+  label: string{length (bytes_of_string label) < 256 - 6} -> // -9?
+  hv: bytes{length hv < 256} ->
+  len: UInt32.t {0 < v len /\ v len <= op_Multiply 255 (hash_length ha)} ->
+  ST (lbytes32 len)
+  (requires (fun h0 -> True))
+  (ensures (fun h0 t h1 -> modifies_none h0 h1))
+
+(*-------------------------------------------------------------------*)
+(*
+  Derive-Secret(Secret, Label, Messages) =
+    HKDF-Expand-Label(Secret, Label,
+       Transcript-Hash(Messages), Hash.length)
+*)
+
+/// used in both hanshakes for deriving intermediate HKDF keys.
+
+val derive_secret:
+  ha: Hashing.Spec.tls_macAlg ->
+  secret: lbytes (Spec.Hash.Definitions.hash_length ha) ->
+  label: string{length (bytes_of_string label) < 256-6} ->
+  digest: bytes{length digest < 256} ->
+  ST (lbytes32 (Hacl.Hash.Definitions.hash_len ha))
+  (requires fun h -> True)
+  (ensures fun h0 _ h1 -> modifies_none h0 h1)
+
