src/tls/MiTLS.HMAC.fsti
@@ -1,0 +1,49 @@
+module MiTLS.HMAC
+
+open MiTLS.Hashing.Spec // for the algorithm names, instead of CoreCrypt
+open MiTLS.Mem
+
+open FStar.HyperStack.ST
+
+let ha = a:EverCrypt.HMAC.supported_alg{Spec.Hash.Definitions.is_md a}
+
+(* Parametric keyed HMAC; could be coded up from two HASH calls. *)
+
+val hmac:
+  a:ha ->
+  k:hkey a ->
+  m:macable a ->
+  Stack (tag a)
+  (requires fun h0 -> True)
+  (ensures fun h0 t h1 ->
+    modifies_none h0 h1 /\
+    t = Hashing.Spec.hmac a k m)
+
+val hmacVerify: a:ha -> k:hkey a -> m:macable a -> t: tag a -> ST (b:bool {b <==> (t == Hashing.Spec.hmac a k m)})
+  (requires (fun h0 -> True))
+  (ensures (fun h0 t h1 -> FStar.HyperStack.modifies Set.empty h0 h1))
+
+(*** Old TLS 1.2 HMAC ***)
+
+/// Agile bytes-friendly MAC function
+
+type macable = b:Bytes.bytes {Bytes.length b + 128 < pow2 32} // [==> pre of hmac for all algorithms]
+
+let tls_mac: a:
+  tls_macAlg ->
+  k: hkey a  ->
+  msg:macable ->
+  ST (tag a)
+  (requires fun h0 -> True)
+  (ensures fun h0 t h1 -> FStar.HyperStack.modifies Set.empty h0 h1) =
+  hmac
+
+let tls_macVerify:
+  a:tls_macAlg ->
+  k: hkey a  ->
+  msg:macable ->
+  tag a ->
+  ST bool
+  (requires fun h0 -> True)
+  (ensures (fun h0 t h1 -> FStar.HyperStack.modifies Set.empty h0 h1)) =
+  hmacVerify
